14MachineCode/Disassemble.thy
@@ -9,50 +9,64 @@ primrec register_map :: "register \<Rightarrow> reg" where
 | "register_map Stk = R4"
 | "register_map Acc = R5"
 
-primrec inv_register_map :: "reg \<Rightarrow> register" where
-  "inv_register_map R1 = Hp"
-| "inv_register_map R2 = Env"
-| "inv_register_map R3 = Vals"
-| "inv_register_map R4 = Stk"
-| "inv_register_map R5 = Acc"
+primrec register_offset :: "register \<Rightarrow> nat" where
+  "register_offset Hp = 0"
+| "register_offset Env = 1"
+| "register_offset Vals = 2"
+| "register_offset Stk = 3"
+| "register_offset Acc = 0"
 
 fun disassemble' :: "assm \<Rightarrow> mach" where
-  "disassemble' (AMov r1 (Reg r2)) = MOV (register_map r1) (register_map r2)"
-| "disassemble' (AMov r1 PC) = MVP (register_map r1)"
-| "disassemble' (AMov r1 (Con k)) = LDI (register_map r1) k"
-| "disassemble' (AGet r1 r2 r3) = LOD (register_map r1) (register_map r3)"
+  "disassemble' (AMov (Reg r)) = MOV R5 (register_map r)"
+| "disassemble' (AMov PC) = MVP R5"
+| "disassemble' (AMov (Con k)) = LDI R5 k"
+| "disassemble' (AGet r1 r2 t) = LOD R5 (register_map r2)"
 | "disassemble' (APut r1 r2 (Reg r3)) = STO (register_map r1) (register_map r3)"
 | "disassemble' (APut r1 r2 PC) = undefined"
 | "disassemble' (APut r1 r2 (Con k)) = STI (register_map r1) k"
-| "disassemble' (ASub r1 k) = SUB (register_map r1) k"
-| "disassemble' (AAdd r1 k) = ADD (register_map r1) k"
+| "disassemble' (ASub Acc k t) = SUB R5 k"
+| "disassemble' (ASub r k t) = SUB (register_map r) (4 * k)"
+| "disassemble' (AAdd Acc k t) = ADD R5 k"
+| "disassemble' (AAdd r k t) = ADD (register_map r) (4 * k)"
 | "disassemble' AJmp = JMP R5"
 
 definition disassemble :: "assm list \<Rightarrow> mach list" where
   "disassemble cd = map disassemble' cd"
 
-fun unmap_mem :: "nat \<Rightarrow> register \<times> nat" where
-  "unmap_mem 0 = (Hp, 0)" 
-| "unmap_mem (Suc 0) = (Env, 0)"
-| "unmap_mem (Suc (Suc 0)) = (Vals, 0)"
-| "unmap_mem (Suc (Suc (Suc 0))) = (Stk, 0)"
-| "unmap_mem (Suc (Suc (Suc (Suc x)))) = (case unmap_mem x of (a, b) \<Rightarrow> (a, Suc b))"
+fun unmap_mem' :: "nat \<Rightarrow> register \<times> nat" where
+  "unmap_mem' 0 = (Hp, 0)" 
+| "unmap_mem' (Suc 0) = (Env, 0)"
+| "unmap_mem' (Suc (Suc 0)) = (Vals, 0)"
+| "unmap_mem' (Suc (Suc (Suc 0))) = (Stk, 0)"
+| "unmap_mem' (Suc (Suc (Suc (Suc x)))) = (case unmap_mem' x of (a, b) \<Rightarrow> (a, Suc b))"
+
+definition unmap_mem :: "(register \<Rightarrow> nat \<Rightarrow> nat) \<Rightarrow> nat \<Rightarrow> nat" where
+  "unmap_mem m x = (case unmap_mem' x of (r, p) \<Rightarrow> m r p)"
+
+fun inv_register_map :: "(register \<Rightarrow> nat) \<Rightarrow> pseudoreg \<Rightarrow> reg \<Rightarrow> nat" where
+  "inv_register_map rs t R1 = rs Hp * 4"
+| "inv_register_map rs t R2 = rs Env * 4 + 1"
+| "inv_register_map rs t R3 = rs Vals * 4 + 2"
+| "inv_register_map rs t R4 = rs Stk * 4 + 3"
+| "inv_register_map rs (Reg r) R5 = rs Acc * 4 + register_offset r"
+| "inv_register_map rs PC R5 = rs Acc"
+| "inv_register_map rs (Con k) R5 = rs Acc"
 
 primrec disassemble_state :: "assm_state \<Rightarrow> mach_state" where
-  "disassemble_state (AS mem rs pc) = MS (rs \<circ> inv_register_map) (uncurry mem \<circ> unmap_mem) pc"
+  "disassemble_state (AS mem rs t pc) = MS (inv_register_map rs t) (unmap_mem mem) pc"
 
-lemma [simp]: "unmap_mem p = (a, b) \<Longrightarrow> uncurry mem (unmap_mem (4 + p)) = mem a (Suc b)"
-  by (simp add: numeral_def split: prod.splits)
+lemma [simp]: "unmap_mem' (4 * k) = (Hp, k)"
+  by (induction k) (simp_all add: numeral_def)
 
-lemma [simp]: "unmap_mem (4 * x) = (Hp, x)"
-  by (induction x rule: unmap_mem.induct) (simp_all add: numeral_def)
+lemma [simp]: "unmap_mem' p = (a, b) \<Longrightarrow> unmap_mem' (4 + p) = (a, Suc b)"
+  by (simp add: numeral_def)
 
 lemma [simp]: "length (disassemble cd) = length cd"
   by (simp add: disassemble_def)
 
 theorem completem [simp]: "cd\<^sub>m \<tturnstile> \<Sigma>\<^sub>m \<leadsto>\<^sub>m \<Sigma>\<^sub>m' \<Longrightarrow> 
   \<exists>cd\<^sub>a \<Sigma>\<^sub>a \<Sigma>\<^sub>a'. cd\<^sub>m = disassemble cd\<^sub>a \<and> disassemble_state \<Sigma>\<^sub>a = \<Sigma>\<^sub>m \<and> 
-    disassemble_state \<Sigma>\<^sub>a' = \<Sigma>\<^sub>m' \<and> iter (\<tturnstile> cd\<^sub>a \<leadsto>\<^sub>a) \<Sigma>\<^sub>a \<Sigma>\<^sub>a'"
+    disassemble_state \<Sigma>\<^sub>a' = \<Sigma>\<^sub>m' \<and> cd\<^sub>a \<tturnstile> \<Sigma>\<^sub>a \<leadsto>\<^sub>a \<Sigma>\<^sub>a'"
 proof (induction cd\<^sub>m \<Sigma>\<^sub>m \<Sigma>\<^sub>m' rule: evalm.induct)
 case (evm_ldi cd pc r k rs mem)
   thus ?case by simp
@@ -82,71 +96,210 @@ next
   thus ?case by simp
 qed
 
-lemma [simp]: "inv_register_map (register_map r) = r"
-  by (induction r) simp_all
-
-lemma [simp]: "register_map (inv_register_map r) = r"
-  by (induction r) simp_all
-
-lemma [simp]: "case_register a b c d e \<circ> inv_register_map = case_reg a b c d e"
-proof 
+lemma inv_reg_map_reg: "r \<noteq> Acc \<Longrightarrow> 
+  (inv_register_map ps act)(R5 := inv_register_map ps act (register_map r)) = 
+    inv_register_map (ps(Acc := ps r)) (Reg r)"
+proof
   fix x
-  show "(case_register a b c d e \<circ> inv_register_map) x = 
-    (case x of R1 \<Rightarrow> a | R2 \<Rightarrow> b | R3 \<Rightarrow> c | R4 \<Rightarrow> d | R5 \<Rightarrow> e)" by (induction x) simp_all
+  show "r \<noteq> Acc \<Longrightarrow> 
+    ((inv_register_map ps act)(R5 := inv_register_map ps act (register_map r))) x = 
+      inv_register_map (ps(Acc := ps r)) (Reg r) x"
+  proof (induction x)
+    case R5
+    thus ?case by (induction r) simp_all
+  qed simp_all
 qed
 
+lemma inv_reg_map_pc: "(inv_register_map ps act)(R5 := pc) = inv_register_map (ps(Acc := pc)) PC"
+proof
+  fix x
+  show "((inv_register_map ps act)(R5 := pc)) x = inv_register_map (ps(Acc := pc)) PC x"
+    by (induction x) simp_all
+qed
+
+lemma inv_reg_map_con: "(inv_register_map ps act)(R5 := k) = 
+  inv_register_map (ps(Acc := k)) (Con 0)"
+proof
+  fix x
+  show "((inv_register_map ps act)(R5 := k)) x = inv_register_map (ps(Acc := k)) (Con 0) x"
+    by (induction x) simp_all
+qed
+
+lemma [simp]: "unmap_mem' (k * 4) = (Hp, k)"
+  by (induction k) (simp_all add: numeral_def)
+
+lemma [simp]: "unmap_mem' (Suc (k * 4)) = (Env, k)"
+  by (induction k) (simp_all add: numeral_def)
+
+lemma [simp]: "unmap_mem' (Suc (Suc (k * 4))) = (Vals, k)"
+  by (induction k) (simp_all add: numeral_def)
+
+lemma [simp]: "unmap_mem' (k * 4 + 3) = (Stk, k)"
+  by (induction k) (simp_all add: numeral_def)
+
+lemma [simp]: "m \<noteq> Acc \<Longrightarrow> unmap_mem' (k * 4 + register_offset m) = (m, k)"
+proof (induction k)
+  case 0
+  thus ?case by (induction m) (simp_all add: numeral_def)
+qed (simp_all add: numeral_def)
+
+lemma [simp]: "r \<noteq> Acc \<Longrightarrow> inv_register_map (ps(r := k)) act R5 = inv_register_map ps act R5"
+  by (induction act) simp_all
+
+lemma [simp]: "r \<noteq> Acc \<Longrightarrow> inv_register_map (ps(r := ps r + k)) act = 
+    ((inv_register_map ps act)(register_map r := inv_register_map ps act (register_map r) + 4 * k))"
+proof
+  fix x
+  show "r \<noteq> Acc \<Longrightarrow> inv_register_map (ps(r := ps r + k)) act x =
+    ((inv_register_map ps act)(register_map r := inv_register_map ps act (register_map r) + 4 * k)) 
+      x" 
+  proof (induction r)
+    case Hp
+    thus ?case by (induction x) simp_all
+  next
+    case Env
+    thus ?case by (induction x) simp_all
+  next
+    case Vals
+    thus ?case by (induction x) simp_all
+  next
+    case Stk
+    thus ?case by (induction x) simp_all
+  next
+    case Acc
+    thus ?case by (induction x) simp_all
+  qed
+qed
+
+lemma [simp]: "r \<noteq> Acc \<Longrightarrow> inv_register_map (ps(r := ps r - k)) act = 
+    ((inv_register_map ps act)(register_map r := inv_register_map ps act (register_map r) - 4 * k))"
+proof
+  fix x
+  show "r \<noteq> Acc \<Longrightarrow> inv_register_map (ps(r := ps r - k)) act x =
+    ((inv_register_map ps act)(register_map r := inv_register_map ps act (register_map r) - 4 * k)) 
+      x" 
+  proof (induction r)
+    case Hp
+    thus ?case by (induction x) simp_all
+  next
+    case Env
+    thus ?case by (induction x) simp_all
+  next
+    case Vals
+    thus ?case by (induction x) simp_all
+  next
+    case Stk
+    thus ?case by (induction x) simp_all
+  next
+    case Acc
+    thus ?case by (induction x) simp_all
+  qed
+qed
+
+lemma [simp]: "m \<noteq> Acc \<Longrightarrow> (r \<noteq> Acc \<Longrightarrow> m = r) \<Longrightarrow>
+    unmap_mem mem (inv_register_map ps (Reg m) (register_map r)) = mem m (ps r)"
+  by (induction r) (simp_all add: unmap_mem_def split: prod.splits)
+
+lemma [simp]: "m \<noteq> Acc \<Longrightarrow> unmap_mem mem (ps Acc * 4 + register_offset m) = mem m (ps Acc)"
+  by (simp add: unmap_mem_def)
+
 theorem correctm [simp]: "cd\<^sub>a \<tturnstile> \<Sigma>\<^sub>a \<leadsto>\<^sub>a \<Sigma>\<^sub>a' \<Longrightarrow>
-   disassemble cd\<^sub>a \<tturnstile> disassemble_state \<Sigma>\<^sub>a \<leadsto>\<^sub>m disassemble_state \<Sigma>\<^sub>a'"
+  disassemble cd\<^sub>a \<tturnstile> disassemble_state \<Sigma>\<^sub>a \<leadsto>\<^sub>m disassemble_state \<Sigma>\<^sub>a'"
 proof (induction cd\<^sub>a \<Sigma>\<^sub>a \<Sigma>\<^sub>a' rule: evala.induct)
-  case (eva_movr cd pc r' r mem ps)
+  case (eva_movr cd pc r mem ps act)
+  hence "disassemble cd ! pc = MOV R5 (register_map r)" by simp
+  hence "disassemble cd \<tturnstile> MS (inv_register_map ps act) (unmap_mem mem) (Suc pc) \<leadsto>\<^sub>m
+    MS ((inv_register_map ps act)(R5 := inv_register_map ps act (register_map r))) 
+      (unmap_mem mem) pc" by simp
+  with eva_movr show ?case by (simp add: inv_reg_map_reg)
+next
+  case (eva_movp cd pc mem ps act)
+  hence "disassemble cd ! pc = MVP R5" by simp
+  hence "disassemble cd \<tturnstile> MS (inv_register_map ps act) (unmap_mem mem) (Suc pc) \<leadsto>\<^sub>m
+    MS ((inv_register_map ps act)(R5 := pc)) (unmap_mem mem) pc" by simp
+  thus ?case by (simp add: inv_reg_map_pc)
+next
+  case (eva_movk cd pc k mem ps act)
+  hence "disassemble cd ! pc = LDI R5 k" by simp
+  hence "disassemble cd \<tturnstile> MS (inv_register_map ps act) (unmap_mem mem) (Suc pc) \<leadsto>\<^sub>m
+    MS ((inv_register_map ps act)(R5 := k)) (unmap_mem mem) pc" by simp
+  thus ?case by (simp add: inv_reg_map_con)
+next
+  case (eva_geta cd pc m t mem ps)
+  hence "disassemble cd ! pc = LOD R5 R5" by simp
+  hence "disassemble cd \<tturnstile> MS (inv_register_map ps (Reg m)) (unmap_mem mem) (Suc pc) \<leadsto>\<^sub>m 
+    MS ((inv_register_map ps (Reg m))(R5 := unmap_mem mem (inv_register_map ps (Reg m) R5))) 
+      (unmap_mem mem) pc" by (metis evm_lod)
+
+  with eva_geta have  "disassemble cd \<tturnstile> 
+    MS (inv_register_map ps (Reg m)) (unmap_mem mem) (Suc pc) \<leadsto>\<^sub>m
+      MS (inv_register_map (ps(Acc := mem m (ps Acc))) t) (unmap_mem mem) pc" by simp
   thus ?case by simp
 next
-  case (eva_movp cd pc r' mem ps)
+  case (eva_get cd pc r t mem ps act)
+  then show ?case try0 by simp
+next
+  case (eva_putr cd pc m r' r mem ps act)
+  then show ?case try0 by simp
+next
+  case (eva_putp cd pc m r' mem ps act)
+  then show ?case try0 by simp
+next
+  case (eva_putk cd pc m r' k mem ps act)
+  then show ?case try0 by simp
+next
+  case (eva_suba cd pc k mem ps act)
+  then show ?case try0 by simp
+next
+  case (eva_sub cd pc r k mem ps act)
+  hence "disassemble cd ! pc = SUB (register_map r) (4 * k)" by simp
+  with eva_sub show ?case by simp
+next
+  case (eva_adda cd pc k mem ps act)
   thus ?case by simp
 next
-  case (eva_movk cd pc r' k mem ps)
-  thus ?case by simp
-next
-  case (eva_get cd pc r' m r mem ps)
-  thus ?case by simp
-next
-  case (eva_putr cd pc m r' r mem ps)
-  thus ?case by simp
-next
-  case (eva_putp cd pc m r' mem ps)
-  thus ?case by simp
-next
-  case (eva_putk cd pc m r' k mem ps)
-  thus ?case by simp
-next
-  case (eva_sub cd pc r k mem ps)
-  thus ?case by simp
-next
-  case (eva_add cd pc r k mem ps)
-  thus ?case by simp
+  case (eva_add cd pc r k mem ps act)
+  hence "disassemble cd ! pc = ADD (register_map r) (4 * k)" by simp
+  with eva_add show ?case by simp
 next
   case (eva_jmp cd pc mem ps)
+  hence "disassemble cd ! pc = JMP R5" by simp
+  hence "disassemble cd \<tturnstile> MS (inv_register_map ps PC) (unmap_mem mem) (Suc pc) \<leadsto>\<^sub>m
+    MS ((inv_register_map ps PC)(R5 := 0)) (unmap_mem mem) (inv_register_map ps PC R5)" 
+      by (metis evm_jmp)
+  hence "disassemble cd \<tturnstile> MS (inv_register_map ps PC) (unmap_mem mem) (Suc pc) \<leadsto>\<^sub>m
+    MS (inv_register_map (ps(Acc := 0)) (Con 0)) (unmap_mem mem) (ps Acc)" by simp
   thus ?case by simp
 qed
 
 theorem correctm_iter [simp]: "iter (\<tturnstile> cd\<^sub>a \<leadsto>\<^sub>a) \<Sigma>\<^sub>a \<Sigma>\<^sub>a' \<Longrightarrow> 
     iter (\<tturnstile> disassemble cd\<^sub>a \<leadsto>\<^sub>m) (disassemble_state \<Sigma>\<^sub>a) (disassemble_state \<Sigma>\<^sub>a')"
   by (induction \<Sigma>\<^sub>a \<Sigma>\<^sub>a' rule: iter.induct) (simp, metis correctm iter_append iter_one)
-
-lemma [simp]: "unmap_mem x = (Stk, 0) \<Longrightarrow> x = 3"
-  by (induction x rule: unmap_mem.induct) (simp_all split: prod.splits)
-
-lemma [simp]: "(uncurry (case_register nmem nmem nmem (nmem(0 := 0, Suc 0 := 0)) nmem) \<circ> 
-  unmap_mem) = (nmem(3 := 0, 7 := 0))"
-proof
-  fix x
-  show "(uncurry (case_register nmem nmem nmem (nmem(0 := 0, Suc 0 := 0)) nmem) \<circ> 
-    unmap_mem) x = (nmem(3 := 0, 7 := 0)) x"
-      by (induction x rule: unmap_mem.induct) 
-         (auto simp add: numeral_def split: prod.splits register.splits)
-qed
-
-lemma [simp]: "case_reg 0 0 0 2 0 = ((\<lambda>r. 0)(R4 := 2))"
+ 
+lemma [simp]: "inv_register_map (case_register 0 0 0 2 0) (Con 0) = case_reg 0 1 2 11 0" 
   by (auto split: reg.splits)
+
+lemma [simp]: "inv_register_map (case_register hp ep (Suc 0) 0 0) (Con 0) = 
+    case_reg (4 * hp) (Suc (4 * ep)) 6 3 0"
+  by (auto split: reg.splits)
+
+lemma [simp]: "unmap_mem' 3 = (Stk, 0)"
+  by (simp add: numeral_def)
+
+lemma [dest]: "unmap_mem' x = (Stk, 0) \<Longrightarrow> x = 3"
+  by (induction x rule: unmap_mem'.induct) (simp_all split: prod.splits)
+
+lemma [simp]: "unmap_mem' 7 = (Stk, 1)"
+  by (simp add: numeral_def)
+
+lemma [dest]: "unmap_mem' x = (Stk, Suc 0) \<Longrightarrow> x = 7"
+  by (induction x rule: unmap_mem'.induct) (auto split: prod.splits)
+
+lemma [simp]: "unmap_mem (case_register nmem nmem nmem (nmem(0 := 0, Suc 0 := 0)) nmem) = 
+    (nmem(3 := 0, 7 := 0))"
+  by rule (auto simp add: unmap_mem_def split: prod.splits register.splits)
+
+lemma [simp]: "unmap_mem (case_register h e v s nmem) 2 = v 0"
+  by (simp add: unmap_mem_def numeral_def)
 
 end
