00Utils/Utils.thy
@@ -96,9 +96,6 @@ proof (induction as arbitrary: bs)
   thus ?case by (induction bs) auto
 qed simp_all
 
-primrec uncurry :: "('a \<Rightarrow> 'b \<Rightarrow> 'c) \<Rightarrow> 'a \<times> 'b \<Rightarrow> 'c" where
-  "uncurry f (a, b) = f a b"
-
 abbreviation nmem :: "nat \<Rightarrow> nat" where
   "nmem x \<equiv> undefined"
 
