Printing.thy
@@ -107,8 +107,8 @@ qed (simp_all add: assemble_heap_def)
 lemma print_u [simp]: "print_uval h p = print_ceclosure (get_closure (H h hp) p)"
   by (cases "h p") simp_all
 
-lemma print_m [simp]: "unmap_mem p = (a, b) \<Longrightarrow> 
-    print_mval (uncurry mem \<circ> unmap_mem) p = print_uval (mem a) b" 
-  by (auto split: nat.splits)
+lemma print_m [simp]: "unmap_mem' p = (a, b) \<Longrightarrow> 
+    print_mval (unmap_mem mem) p = print_uval (mem a) b" 
+  by (auto simp add: unmap_mem_def split: nat.splits)
 
 end
